tests/cpp2v-parser/test13.cpp
@@ -1,0 +1,13 @@
+enum X { Y , Z };
+
+enum A : int { B , C };
+
+
+typedef X TD;
+typedef A TE;
+
+#if 0
+typedef enum { U } Unit;
+
+typedef enum { V } unit;
+#endif
