tests/cpp2v-parser/test14.cpp
@@ -1,0 +1,21 @@
+struct S {};
+
+int f(int &x) { return x; }
+int g(int x) { return x; }
+
+void fS(S &x) { }
+void gS(S x) { }
+void hS(S *x) { }
+
+int main() {
+  int x;
+  f(x);
+  g(x);
+
+  S s;
+  fS(s);
+  gS(s);
+  hS(&s);
+
+  return 1;
+}
