theories/Sem/Semantics.v
@@ -8,12 +8,13 @@ From Cpp Require Import
      Ast.
 
 (** values *)
+Parameter val : Type.
+
 Parameter ptr : Type.
 
-(** values *)
-Parameter val : Type.
 Parameter Vptr : ptr -> val.
 Parameter Vint : Z -> val.
+
 
 (* todo(gmm): maintain stack variables through regions
  *)
@@ -26,18 +27,17 @@ Axiom has_type_int : forall z,
 Axiom has_type_int32 : forall z,
     (-Z.pow 2 31 < z < Z.pow 2 31 - 1)%Z ->
     has_type (Vint z) T_int32.
-Axiom has_type_qual : forall v q ty,
-    has_type v ty -> has_type v (Tqualified q ty).
 
 (* this is an axiom *)
 Axiom has_type_int_any : forall x, has_type (Vint x) T_int.
-Axiom has_type_int_bound : forall {q x},
-    has_type (Vint x) (Tqualified q T_int) ->
+Axiom has_type_int_bound : forall {x},
+    has_type (Vint x) T_int ->
     (-(2^31) < x < 2^31 - 1)%Z.
+Axiom has_type_qual : forall t q x,
+    has_type x (drop_qualifiers t) ->
+    has_type x (Tqualified q t).
 
-Axiom has_type_mut : forall x ty, has_type x ty -> has_type x (Qmut ty).
-
-Hint Resolve has_type_int_any has_type_int_bound has_type_mut
+Hint Resolve has_type_int_any has_type_int_bound has_type_qual
   : has_type.
 
 
